code/experimental/sparkle/Hacl.SPARKLE.fst
@@ -1,0 +1,33 @@
+module Hacl.SPARKLE
+
+open FStar.Mul
+open FStar.HyperStack
+open FStar.HyperStack.ST
+
+open Lib.IntTypes
+open Lib.Buffer
+
+#set-options "--max_fuel 0 --max_ifuel 0"
+
+module Spec = Spec.SPARKLE
+
+type branch = lbuffer uint32 (size 2)
+let branch_to_spec (b: branch) (h : mem) : GTot Spec.branch =
+  let b_values = as_seq h b in
+  (Seq.index b_values 0, Seq.index b_values 1)
+
+
+val arx: c:uint32 -> b:branch -> Stack unit
+  (requires (fun h0 ->
+    live h0 b
+  ))
+  (ensures (fun h0 new_b h1 ->
+    branch_to_spec b h1 == Spec.arx c (branch_to_spec b h0) /\
+    modifies1 b h0 h1
+  ))
+let arx c b =
+  let x = index b (size 0) in
+  let y = index b (size 1) in
+  let x, y = Spec.arx c (x,y) in
+  upd b (size 0) x;
+  upd b (size 1) y
